\documentclass{article}
\usepackage{epsfig}
\pagestyle{empty}
\begin{document}
\begin{eqnarray*}{ R^1 & = & (R_2-R_1)*\frac{x-x_1}{x_2-x_1}+R_1 \\ R^2 & = & (R_3-R_1)*\frac{x-x_1}{x_3-x_1}+R_1 \\ \ldots \\ R^{10} & = & (R_5-R_4)*\frac{x-x_4}{x_5-x_4}+R_4 \end{eqnarray*}{
\pagebreak

$ R $
\pagebreak

$ G $
\pagebreak

$ y $
\pagebreak

$ B $
\pagebreak

$ z $
\pagebreak

$ \alpha $
\pagebreak

$ w $
\pagebreak

$ R^2 $
\pagebreak

$ z^2 $
\pagebreak

$ z^3 $
\pagebreak

$ e^{-\alpha*z^2} $
\pagebreak

$ C \rightarrow C $
\pagebreak

\begin{eqnarray*}{ F_0 & = & Real(z) \\ F_1 & = & Imag(z) \\ F_2 & = & Real(f(z)) \\ F_3 & = & Imag(f(z)) \end{eqnarray*}{
\pagebreak

$ f(z) = z^2 $
\pagebreak

$ f(z) = z^3 $
\pagebreak

$ f(z) = z^\alpha $
\pagebreak

$ f(z) = e^{\alpha*z} $
\pagebreak

$ f(z) = e^{-\alpha*z^2} $
\pagebreak

$ f(z) = \frac{1}{z} $
\pagebreak

$ f(z) = \frac{1}{z^2} $
\pagebreak

$ f(z) = \sqrt{z} $
\pagebreak

$ f(z) = \ln{z} $
\pagebreak

$ f(z) = \sin{z} $
\pagebreak

$ f(z) = \cos{z} $
\pagebreak

$ f(z) = \sinh{z} $
\pagebreak

$ f(z) = \cosh{z} $
\pagebreak

$ f(z) = \tan{z} $
\pagebreak

$ f: R^3 \rightarrow R $
\pagebreak

$ r = r(\psi, \theta, \phi) $
\pagebreak

$ f: R^2 \rightarrow R^4 $
\pagebreak

$ f: C \rightarrow C $
\pagebreak

\[ \frac{df}{dt} = \lim_{h \rightarrow 0} \frac{f(t+h, u, v) - f(t, u, v)}{h}, \frac{df}{du},\frac{df}{dv}\mbox{analogously} \]
\pagebreak

$ 3^4 $
\pagebreak

$ R^3 $
\pagebreak

$ R^4 $
\pagebreak

$ \vec{x} = ( x, y, z, f(x, y, z) ) $
\pagebreak

\begin{eqnarray*} { F_0 & = & Radius*\sin(\psi)*\sin(\theta)*\cos(\phi) \\ F_1 & = & Radius*\sin(\psi)*\sin(\theta)*\sin(\phi) \\ F_2 & = & Radius*\sin(\psi)*\cos(\theta) \\ F_3 & = & Radius*\cos(\psi) \end{eqnarray*}
\pagebreak

$R^3 \rightarrow R$
\pagebreak

\begin{eqnarray*}{ r^2 & = & x^2+y^2+z^2 \\ f(x,y,z) & = & 1./(r^2+.25) \end{eqnarray*}{
\pagebreak

$ f(x,y,z) = \sin (\pi*(x^2+y^2+z^2)) $
\pagebreak

$ f(x,y,z) = \exp (x^2+y^2+z^2) $
\pagebreak

$ r(\psi, \theta, \phi) = |\sin (Phase*\pi*\psi*\theta*\phi)| $
\pagebreak

$ r = \sin(\pi/3.*(\psi+\theta+\phi)) $
\pagebreak

$ r = \sqrt{\psi^2+\theta^2+\phi^2} $
\pagebreak

\[ \frac{df}{du} = \lim_{h \rightarrow 0} \frac{f(u+h, v) - f(u, v)}{h}, \frac{df}{dv}\mbox{analogously} \]
\pagebreak

$ R^2 \rightarrow R^4 $
\pagebreak

\begin{eqnarray*}{ F_0 & = & Radius*\sin \theta*\sin \psi; \\ F_1 & = & Radius*\cos \theta*\sin \psi; \\ F_2 & = & Radius*\cos \theta; \\ F_3 & = & Radius*\cos \psi; \end{eqnarray*}{
\pagebreak

\begin{eqnarray*}{ t & = & \theta*\pi \\ p & = & \phi*frac{\pi}{2} \\ F_0 & = (1-\sin{t})*\cos{p} \\ F_1 & = (1-\sin{t})*\sin{p} \\ F_2 & = (1+\sin{t})*\cos{p} \\ F_3 & = (1+\sin{t})*\sin{p} \\ F & = & F*\frac{1}{\sqrt{2}}*\cos{t} \end{eqnarray*}{
\pagebreak

$ D-1 $
\pagebreak

$ D $
\pagebreak

$ X_{new}_{D-1} = \frac{X_{D-1} }{2} $
\pagebreak

$ X_{new}_{D-1} $
\pagebreak

$ X_{D-2} $
\pagebreak

$ D-2 $
\pagebreak

$ \sqrt{1 - \bar{x_i}^2} $
\pagebreak

$ \bar{x_i} $
\pagebreak

$ \frac{1}{2} $
\pagebreak

$ \sqrt{x_{D-1} }^2 - \frac{1}{2^2} } $
\pagebreak

$ R^3 \rightarrow R $
\pagebreak

$ \vec{x} = f(\theta, \phi, \psi) $
\pagebreak

$ M_{ij} $
\pagebreak

\end{document}
